Clean out FutureEtaExpand

Launchbury/FutureEtaExpand.thy
@@ -1,221 +1,16 @@
 theory FutureEtaExpand
-imports CallFutures AEnv Terms EtaExpansionArity EtaExpansionSestoft AbstractTransform Set_Cpo_Nominal  Sestoft SestoftGC ArityAnalysisAbinds
+imports CardinalityAnalysis AbstractTransform Sestoft SestoftGC  ArityEtaExpansionSestoft
 begin
 
 default_sort type
 
-type_synonym oneShot = "one"
-abbreviation notOneShot :: oneShot where "notOneShot \<equiv> ONE"
-abbreviation oneShot :: oneShot where "oneShot \<equiv> \<bottom>"
-
-type_synonym two = "oneShot\<^sub>\<bottom>"
-abbreviation many :: two where "many \<equiv> up\<cdot>notOneShot"
-abbreviation once :: two where "once \<equiv> up\<cdot>oneShot"
-abbreviation none :: two where "none \<equiv> \<bottom>"
-
-lemma two_conj: "c = many \<or> c = once \<or> c = none" by (metis Exh_Up one_neq_iffs(1))
-
-lemma two_cases[case_names many once none]:
-  obtains "c = many" | "c = once" | "c = none" using two_conj by metis
-
-definition two_pred where "two_pred = (\<Lambda> x. if x \<sqsubseteq> once then \<bottom> else x)"
-
-lemma two_pred_simp: "two_pred\<cdot>c = (if c \<sqsubseteq> once then \<bottom> else c)"
-  unfolding two_pred_def
-  apply (rule beta_cfun)
-  apply (rule cont_if_else_above)
-  apply (auto elim: below_trans)
-  done
-
-lemma two_pred_below_arg: "two_pred \<cdot> f \<sqsubseteq> f"
-  by (auto simp add: two_pred_simp)
-
-lemma two_pred_none: "two_pred\<cdot>c = none \<longleftrightarrow> c \<sqsubseteq> once"
-  by (auto simp add: two_pred_simp)
-
-definition record_call where "record_call x = (\<Lambda> ce. (\<lambda> y. if x = y then two_pred\<cdot>(ce y) else ce y))"
-
-lemma record_call[simp]: "(record_call x \<cdot> f) x = two_pred \<cdot> (f x)"
-  unfolding record_call_def by auto
-
-lemma record_call_below_arg: "record_call x \<cdot> f \<sqsubseteq> f"
-  unfolding record_call_def
-  by (auto intro!: fun_belowI two_pred_below_arg)
-
-
-definition abstractPath :: "var list set \<Rightarrow> var \<Rightarrow> two"
-  where "abstractPath ps v = undefined"
-
-(*
-text {* Expands only if it is safe to do so, i.e. either one-shot or already a function. *}
-
-fun rhsExpand :: "(Arity \<times> one) \<Rightarrow> exp \<Rightarrow> exp"
-  where "rhsExpand (a,c) e = (if isLam e \<or> c = \<bottom> then Aeta_expand a e else e)"
-
-interpretation supp_bounded_transform rhsExpand sorry
-
-lemma rhsExpand[eqvt]: "\<pi> \<bullet> rhsExpand = rhsExpand" sorry
-*)
-
-fun Astack :: "stack \<Rightarrow> Arity"
-  where "Astack [] = 0"
-      | "Astack (Arg x # S) = inc\<cdot>(Astack S)"
-      | "Astack (Upd x # S) = 0"
-      | "Astack (Dummy x # S) = 0"
-
-fun upds_list :: "stack \<Rightarrow> var list" where
-  "upds_list [] = []"
-| "upds_list (Upd x # S) = x # upds_list S"
-| "upds_list (Arg x # S) = upds_list S"
-| "upds_list (Dummy x # S) = upds_list S"
-
-lemma set_upds_list[simp]:
-  "set (upds_list S) = upds S"
-  by (induction S rule: upds_list.induct) auto
-
-fun heap_upds_ok where "heap_upds_ok (\<Gamma>,S) \<longleftrightarrow> domA \<Gamma> \<inter> upds S = {} \<and> distinct (upds_list S)"
-
-lemma heap_upds_okE: "heap_upds_ok (\<Gamma>, S) \<Longrightarrow> x \<in> domA \<Gamma> \<Longrightarrow> x \<notin> upds S"
-  by auto
-
-lemma heap_upds_ok_app1: "heap_upds_ok (\<Gamma>, S) \<Longrightarrow> heap_upds_ok (\<Gamma>,Arg x # S)" by auto
-lemma heap_upds_ok_app2: "heap_upds_ok (\<Gamma>, Arg x # S) \<Longrightarrow> heap_upds_ok (\<Gamma>, S)" by auto
-
-lemma heap_upds_ok_append:
-  assumes "domA \<Delta> \<inter> domA \<Gamma> = {}"
-  assumes "domA \<Delta> \<inter> upds S = {}"
-  assumes "heap_upds_ok (\<Gamma>,S)"
-  shows "heap_upds_ok (\<Delta>@\<Gamma>, S)"
-  using assms
-  unfolding heap_upds_ok.simps
-  by auto
-
-lemma heap_upds_ok_to_stack:
-  "x \<in> domA \<Gamma> \<Longrightarrow> heap_upds_ok (\<Gamma>, S) \<Longrightarrow> heap_upds_ok (delete x \<Gamma>, Upd x #S)"
-  by (auto)
-
-lemma heap_upds_ok_to_heap:
-  "heap_upds_ok (\<Gamma>, Upd x # S) \<Longrightarrow> heap_upds_ok ((x,e) # \<Gamma>, S)"
-  by (auto)
-
-lemma heap_upds_ok_reorder:
-  "x \<in> domA \<Gamma> \<Longrightarrow> heap_upds_ok (\<Gamma>, S) \<Longrightarrow> heap_upds_ok ((x,e) # delete x \<Gamma>, S)"
-  by (intro heap_upds_ok_to_heap heap_upds_ok_to_stack)
-
-lemmas heap_upds_ok_intros[intro] = heap_upds_ok_to_heap heap_upds_ok_to_stack heap_upds_ok_reorder heap_upds_ok_app1 heap_upds_ok_app2
-lemmas heap_upds_ok.simps[simp del]
-
-lemma Aeta_expand_correct:
-  assumes "Astack S \<sqsubseteq> a"
-  shows "(\<Gamma>, Aeta_expand a e, S) \<Rightarrow>\<^sup>* (\<Gamma>, e, S)"
-proof-
-  have "arg_prefix S = Rep_Arity (Astack S)"
-    by (induction S arbitrary: a rule: arg_prefix.induct) (auto simp add: Arity.zero_Arity.rep_eq[symmetric])
-  also
-  from assms(1)
-  have "Rep_Arity a \<le> Rep_Arity (Astack S)" by (metis below_Arity.rep_eq)
-  finally
-  show ?thesis by transfer (rule eta_expansion_correct')
-qed
-
-
-fun restr_stack :: "var set \<Rightarrow> stack \<Rightarrow> stack"
-  where "restr_stack V [] = []"
-      | "restr_stack V (Arg x # S) = Arg x # restr_stack V S"
-      | "restr_stack V (Upd x # S) = (if x \<in> V then Upd x # restr_stack V S else restr_stack V S)"
-      | "restr_stack V (Dummy x # S) = Dummy x # restr_stack V S"
-
-lemma Astack_restr_stack_below:
-  "Astack (restr_stack V S) \<sqsubseteq> Astack S"
-  by (induction V S rule: restr_stack.induct) auto
-
-lemma restr_stack_cong:
-  "(\<And> x. x \<in> upds S \<Longrightarrow> x \<in> V \<longleftrightarrow> x \<in> V') \<Longrightarrow> restr_stack V S = restr_stack V' S"
-  by (induction V S rule: restr_stack.induct) auto
-
-lemma upds_restr_stack[simp]: "upds (restr_stack V S) = upds S \<inter> V"
-  by (induction V S rule: restr_stack.induct) auto
-
-lemma fresh_star_restict_stack[intro]:
-  "a \<sharp>* S \<Longrightarrow> a \<sharp>* restr_stack V S"
-  by (induction V S rule: restr_stack.induct) (auto simp add: fresh_star_Cons)
-
-definition fup_fst :: "(var \<Rightarrow> (Arity \<times> one)\<^sub>\<bottom>) \<Rightarrow> AEnv"
-    where "fup_fst e x = fup\<cdot>(\<Lambda> p. up\<cdot>(cfst\<cdot>p))\<cdot>(e x)"
-
-lemma fup_fst_eqvt[eqvt]: "\<pi> \<bullet> (fup_fst e x) = fup_fst (\<pi> \<bullet> e) (\<pi> \<bullet> x)"
-  unfolding fup_fst_def
-  by perm_simp rule
-
-definition const_on :: "('a \<Rightarrow> 'b) \<Rightarrow> 'a set \<Rightarrow> 'b \<Rightarrow> bool"
-  where "const_on f S x = (\<forall> y \<in> S . f y = x)"
-
-lemma const_on_simp:
- "const_on f S r \<Longrightarrow> x \<in> S \<Longrightarrow> f x = r"
- by (simp add: const_on_def)
-
-lemma const_onE[elim]: "const_on f S r ==> x : S ==> r = r' ==> f x = r'"     by (simp add: const_on_def)
-
-lemma const_on_insert[simp]: "const_on f (insert x S) y \<longleftrightarrow> const_on f S y \<and> f x = y"
-  unfolding const_on_def by auto
-
-context ArityAnalysis 
-begin
-  abbreviation "aExp \<equiv> Aexp"
-end
-
-locale FutureAnalysis = ArityAnalysis +
-  fixes aHeap :: "heap \<Rightarrow> exp \<Rightarrow> Arity \<rightarrow> AEnv"
-  fixes fHeap :: "heap \<Rightarrow> exp \<Rightarrow> Arity \<rightarrow> (var \<Rightarrow> two)"
-
-  assumes aExp[eqvt]: "\<pi> \<bullet> aExp = aExp"
-  assumes aExp_Var: "up \<cdot> n \<sqsubseteq> (aExp (Var x)\<cdot>n) x"
-  assumes aExp_App: "aExp (App e x) \<cdot> n = aExp e \<cdot>(inc\<cdot>n) \<squnion> AE_singleton x \<cdot> (up\<cdot>0)"
-  assumes aExp_subst_App_Lam: "aExp (e[y::=x]) \<sqsubseteq> aExp (App (Lam [y]. e) x)"
-  assumes aExp_Lam: "aExp (Lam [y]. e) \<cdot> n = env_delete y (aExp e \<cdot>(pred\<cdot>n))"
-
-  assumes aExp_Subst: "aExp (Lam [y]. e)\<cdot>a \<sqsubseteq> ae \<Longrightarrow> ae x = up\<cdot>0 \<Longrightarrow> aExp (e[y::=x])\<cdot>(pred\<cdot>a) \<sqsubseteq> ae"
-
-
-
-
-  assumes aHeap_eqvt[eqvt]: "\<pi> \<bullet> aHeap = aHeap"
-  assumes edom_aHeap: "edom (aHeap \<Gamma> e\<cdot> a) \<subseteq> domA \<Gamma>"
-  assumes aHeap_heap3: "x \<in> thunks \<Gamma> \<Longrightarrow> many \<sqsubseteq> (fHeap \<Gamma> e\<cdot>a) x \<Longrightarrow> (aHeap \<Gamma> e\<cdot>a) x = up\<cdot>0"
-  assumes aHeap_subst: "x \<notin> domA \<Gamma> \<Longrightarrow> y \<notin> domA \<Gamma> \<Longrightarrow> aHeap \<Gamma>[x::h=y] e[x ::=y]  = aHeap \<Gamma> e"
-
-
-  assumes aExp_Let: "ABinds \<Gamma>\<cdot>(aHeap \<Gamma> e\<cdot>a) \<squnion> aExp e\<cdot>a \<sqsubseteq> aHeap \<Gamma> e\<cdot>a \<squnion>  aExp (Let \<Gamma> e)\<cdot>a"
-  (*
-  assumes aHeap_heap: "map_of \<Gamma> x = Some e' \<Longrightarrow>  fup\<cdot>(aExp e')\<cdot>((aHeap \<Gamma> e\<cdot>a) x) f|` domA \<Gamma> \<sqsubseteq> aHeap \<Gamma> e\<cdot>a"
-  assumes aHeap_heap2: "map_of \<Gamma> x = Some e' \<Longrightarrow> fup\<cdot>(aExp e')\<cdot>((aHeap \<Gamma> e\<cdot>a) x) f|` (- domA \<Gamma>) \<sqsubseteq>  aExp (Let \<Gamma> e)\<cdot>a"
-  assumes aHeap_above_aExp: "aExp e\<cdot>a f|` domA \<Gamma> \<sqsubseteq> aHeap \<Gamma> e\<cdot>a"
-  assumes aExp_Let_above:   "aExp e\<cdot>a f|` (- domA \<Gamma>) \<sqsubseteq> aExp (Let \<Gamma> e)\<cdot>a"
-  *)
- 
-  assumes fHeap[eqvt]: "\<pi> \<bullet> fHeap = fHeap"
-  assumes edom_fHeap[simp]: "edom (fHeap \<Delta> e\<cdot>a) = edom (aHeap \<Delta> e\<cdot>a)"
-
-  fixes prognosis :: "AEnv \<Rightarrow> Arity \<Rightarrow> conf \<Rightarrow> (var \<Rightarrow> two)"
-    (*    where "prognosis ae a (\<Gamma>, e, S) = abstractPath (paths (anal_env fExp \<Gamma> \<cdot> ae) (fstack S \<cdot>(fExp e \<cdot> a)))" *)
-
-  assumes prognosis_App: "prognosis ae (inc\<cdot>a) (\<Gamma>, e, Arg x # S) \<sqsubseteq> prognosis ae a (\<Gamma>, App e x, S)"
-  assumes prognosis_subst_Lam: "prognosis ae (pred\<cdot>a) (\<Gamma>, e[y::=x], S) \<sqsubseteq> prognosis ae a (\<Gamma>, Lam [y]. e, Arg x # S)"
-  assumes prognosis_Var: "ae x = up\<cdot>u \<Longrightarrow> a \<sqsubseteq> u \<Longrightarrow> prognosis ae u (delete x \<Gamma>, e, Upd x # S) \<sqsubseteq> record_call x \<cdot> (prognosis ae a (\<Gamma>, Var x, S))"
-  assumes prognosis_Var2: "ae x \<sqsubseteq> up\<cdot>a \<Longrightarrow> prognosis ae a ((x, e) # \<Gamma>, e, S) \<sqsubseteq> prognosis ae a (\<Gamma>, e, Upd x # S)"
-  assumes prognosis_Let: "prognosis (aHeap \<Delta> e\<cdot>a \<squnion> ae) a (\<Delta> @ \<Gamma>, e, S) \<sqsubseteq> fHeap \<Delta> e\<cdot>a \<squnion> prognosis ae a (\<Gamma>, Terms.Let \<Delta> e, S)"
-
-  assumes prognosis_ap: "const_on (prognosis ae a (\<Gamma>, e, S)) (ap S) many"
-  assumes prognosis_env_cong: "ae f|` domA \<Gamma> = ae' f|` domA \<Gamma> \<Longrightarrow> prognosis ae u (\<Gamma>, e, S) = prognosis ae' u (\<Gamma>, e, S)"
-
-  assumes artiy_edom_prognosis: "edom (ABinds \<Gamma>\<cdot>ae \<squnion> aExp e\<cdot>a) \<subseteq> edom (prognosis ae a (\<Gamma>, e, S))"
-
+locale CardinalityArityTransformation = CardinalityPrognosisEdom + CardinalityPrognosisCorrectLet 
 begin
 
   sublocale AbstractTransformBound
     "\<lambda> a . inc\<cdot>a"
     "\<lambda> a . pred\<cdot>a"
-    "\<lambda> \<Delta> e a . (a, aHeap \<Delta> e\<cdot>a)"
+    "\<lambda> \<Delta> e a . (a, Aheap \<Delta> e\<cdot>a)"
     "fst"
     "snd"
     "Aeta_expand"
@@ -227,13 +22,13 @@ begin
   sublocale AbstractTransformBoundSubst
     "\<lambda> a . inc\<cdot>a"
     "\<lambda> a . pred\<cdot>a"
-    "\<lambda> \<Delta> e a . (a, aHeap \<Delta> e\<cdot>a)"
+    "\<lambda> \<Delta> e a . (a, Aheap \<Delta> e\<cdot>a)"
     "fst"
     "snd"
     "Aeta_expand"
     "snd"
   apply default
-  apply (simp add: aHeap_subst)
+  apply (simp add: Aheap_subst)
   apply (rule subst_Aeta_expand)
   done
 
@@ -247,16 +42,6 @@ begin
 
   type_synonym tstate = "(AEnv \<times> (var \<Rightarrow> two) \<times> Arity)"
 
-  fixrec u_com :: "'a::cpo\<^sub>\<bottom> \<rightarrow> 'b::cpo\<^sub>\<bottom> \<rightarrow> ('a \<times> 'b)\<^sub>\<bottom>"
-    where "u_com\<cdot>(up\<cdot>x)\<cdot>(up\<cdot>y) = up\<cdot>(x, y)"
-  lemma u_com_strict[simp]: "u_com\<cdot>\<bottom>\<cdot>\<bottom> = \<bottom>" by fixrec_simp
-
-  definition env_u_com ::  "('c::type \<Rightarrow> 'a::cpo\<^sub>\<bottom>) \<Rightarrow> ('c \<Rightarrow> 'b::cpo\<^sub>\<bottom>) \<Rightarrow> ('c \<Rightarrow> ('a \<times> 'b)\<^sub>\<bottom>)"
-    where [simp]: "env_u_com e1 e2 x = u_com\<cdot>(e1 x)\<cdot>(e2 x)"
-  lemma env_u_com_delete: "env_u_com (env_delete x e1) (env_delete x e2) = env_delete x (env_u_com e1 e2)"
-    by (rule, case_tac "xa = x") auto
-  
-
   fun conf_transform :: "tstate \<Rightarrow> conf \<Rightarrow> conf"
   where "conf_transform (ae, ce,  a) (\<Gamma>, e, S) =
     (restrictA (edom ae) (map_transform Aeta_expand ae (map_transform ccTransform ae \<Gamma>)), 
@@ -266,13 +51,6 @@ begin
   definition anal_env :: "(exp \<Rightarrow> 'a::cpo \<rightarrow> 'b::pcpo) \<Rightarrow> heap \<Rightarrow> (var \<Rightarrow> 'a\<^sub>\<bottom>) \<rightarrow> (var \<Rightarrow> 'b)"
     where "anal_env f \<Gamma> = (\<Lambda> e. (\<lambda> x . fup\<cdot>(f (the (map_of \<Gamma> x)))\<cdot>(e x)))"
 
-  fun fstack :: "stack \<Rightarrow> future set \<rightarrow> future set"
-    where "fstack [] = (\<Lambda> f. f)"
-        | "fstack (Arg x # S) = (\<Lambda> f . fstack S \<cdot> (may_call x f))"
-        | "fstack (Upd x # S) = fstack S"
-        | "fstack (Dummy x # S) = fstack S"
-
-
   inductive consistent :: "tstate \<Rightarrow> conf \<Rightarrow> bool" where
     consistentI[intro!]: 
     "edom ae \<subseteq> domA \<Gamma> \<union> upds S
@@ -280,17 +58,13 @@ begin
     \<Longrightarrow> edom ce = edom ae
     \<Longrightarrow> Astack (restr_stack (edom ae) S) \<sqsubseteq> a
     \<Longrightarrow> prognosis ae a (\<Gamma>, e, S) \<sqsubseteq> ce
-    \<Longrightarrow> ABinds \<Gamma>\<cdot>ae \<squnion> aExp e\<cdot>a \<sqsubseteq> ae
+    \<Longrightarrow> ABinds \<Gamma>\<cdot>ae \<squnion> Aexp e\<cdot>a \<sqsubseteq> ae
     \<Longrightarrow> (\<And> x. x \<in> thunks \<Gamma> \<Longrightarrow>  many \<sqsubseteq> ce x \<Longrightarrow> ae x = up\<cdot>0)
     \<Longrightarrow> const_on ae (ap S) (up\<cdot>0)
     \<Longrightarrow> const_on ae (upds (restr_stack (edom ae) S)) (up\<cdot>0)
     \<Longrightarrow> consistent (ae, ce, a) (\<Gamma>, e, S)"  
   inductive_cases consistentE[elim!]: "consistent (ae, ce, a) (\<Gamma>, e, S)"
   
-  lemma isLam_transform[simp]:
-    "isLam (transform a e) \<longleftrightarrow> isLam e"
-    by (induction e rule:isLam.induct) (case_tac b, auto)
-
   lemma foo:
     fixes c c' R 
     assumes "c \<Rightarrow>\<^sup>* c'" and "\<not> boring_step c'" and "consistent (ae,ce,a) c"
@@ -300,7 +74,7 @@ begin
   case (app\<^sub>1 \<Gamma> e x S)
     have "prognosis ae (inc\<cdot>a) (\<Gamma>, e, Arg x # S) \<sqsubseteq> prognosis ae a (\<Gamma>, App e x, S)" by (rule prognosis_App)
     with app\<^sub>1 have "consistent (ae, ce, inc\<cdot>a) (\<Gamma>, e, Arg x # S)"
-      by (auto simp add: join_below_iff aExp_App  elim: below_trans)
+      by (auto simp add: join_below_iff  dest!: below_trans[OF Aexp_App] elim: below_trans)
     moreover
     have "conf_transform (ae, ce, a) (\<Gamma>, App e x, S) \<Rightarrow>\<^sub>G conf_transform (ae, ce, inc\<cdot>a) (\<Gamma>, e, Arg x # S)"
       by simp rule
@@ -310,9 +84,18 @@ begin
 case (app\<^sub>2 \<Gamma> y e x S)
   have "prognosis ae (pred\<cdot>a) (\<Gamma>, e[y::=x], S) \<sqsubseteq> prognosis ae a (\<Gamma>, (Lam [y]. e), Arg x # S)"
      by (rule prognosis_subst_Lam)
-  then
-  have "consistent (ae, ce, pred\<cdot>a) (\<Gamma>, e[y::=x], S)"  using app\<^sub>2
-    by (auto elim: below_trans edom_mono elim: aExp_Subst simp add: join_below_iff)
+  moreover
+  {
+  have "Aexp (e[y::=x])\<cdot>(pred\<cdot>a) \<sqsubseteq> env_delete y ((Aexp e)\<cdot>(pred\<cdot>a)) \<squnion> AE_singleton x\<cdot>(up\<cdot>0)" by (rule Aexp_Subst)
+  also have "env_delete y ((Aexp e)\<cdot>(pred\<cdot>a)) \<sqsubseteq> Aexp (Lam [y]. e)\<cdot>a" by (rule Aexp_Lam)
+  also have "\<dots> \<sqsubseteq> ae" using app\<^sub>2 by (auto simp add: join_below_iff)
+  also have "AE_singleton x\<cdot>(up\<cdot>0) \<sqsubseteq> ae" using app\<^sub>2 by auto
+  also have "ae \<squnion> ae = ae" by simp
+  finally  have "Aexp (e[y::=x])\<cdot>(pred\<cdot>a) \<sqsubseteq> ae" by this simp_all
+  }
+  ultimately
+  have "consistent (ae, ce, pred\<cdot>a) (\<Gamma>, e[y::=x], S)" using app\<^sub>2
+    by (auto elim: below_trans edom_mono  simp add: join_below_iff)
   moreover
   have "conf_transform (ae, ce, a) (\<Gamma>, Lam [y]. e, Arg x # S) \<Rightarrow>\<^sub>G conf_transform (ae, ce, pred \<cdot> a) (\<Gamma>, e[y::=x], S)" by (simp add: subst_transform[symmetric]) rule
   ultimately
@@ -323,8 +106,8 @@ case (thunk \<Gamma> x e S)
   hence [simp]: "x \<in> domA \<Gamma>" by (rule set_mp[OF thunks_domA])
   hence "x \<notin> upds S" using thunk by (auto elim!: heap_upds_okE)
 
-  from thunk have "aExp (Var x)\<cdot>a \<sqsubseteq> ae" by (auto simp add: join_below_iff)
-  from below_trans[OF aExp_Var fun_belowD[OF this] ]
+  from thunk have "Aexp (Var x)\<cdot>a \<sqsubseteq> ae" by (auto simp add: join_below_iff)
+  from below_trans[OF Aexp_Var fun_belowD[OF this] ]
   have "up\<cdot>a \<sqsubseteq> ae x".    
   then obtain u where "ae x = up\<cdot>u" and "a \<sqsubseteq> u" by (cases "ae x") auto
   hence [simp]: "x \<in> edom ae" by (simp add: edom_def)
@@ -332,9 +115,9 @@ case (thunk \<Gamma> x e S)
   have "Astack (restr_stack (edom ae) S) \<sqsubseteq> u" using thunk `a \<sqsubseteq> u` by (auto elim: below_trans)
 
   from Abinds_reorder1[OF `map_of \<Gamma> x = Some e`] `ae x = up\<cdot>u`
-  have "ABinds (delete x \<Gamma>)\<cdot>ae \<squnion> aExp e\<cdot>u = ABinds \<Gamma>\<cdot>ae" by (auto intro: join_comm)
+  have "ABinds (delete x \<Gamma>)\<cdot>ae \<squnion> Aexp e\<cdot>u = ABinds \<Gamma>\<cdot>ae" by (auto intro: join_comm)
   also have "\<dots> \<sqsubseteq> ae" using thunk by (auto simp add: join_below_iff)
-  finally have "ABinds (delete x \<Gamma>)\<cdot>ae \<squnion> aExp e\<cdot>u \<sqsubseteq> ae".
+  finally have "ABinds (delete x \<Gamma>)\<cdot>ae \<squnion> Aexp e\<cdot>u \<sqsubseteq> ae".
 
   show ?case
   proof(cases "ce x" rule:two_cases)
@@ -351,7 +134,7 @@ case (thunk \<Gamma> x e S)
     have "prognosis ae a (\<Gamma>, Var x, S) \<sqsubseteq> ce" using thunk by auto
     hence "prognosis ae a (\<Gamma>, Var x, S) x \<sqsubseteq> once"
       using once by (metis (mono_tags) fun_belowD)
-    hence "x \<notin> ap S" using prognosis_ap by (auto simp add: const_on_def)
+    hence "x \<notin> ap S" using prognosis_ap[of ae a \<Gamma> "(Var x)" S] by auto
     
 
     from `ae x = up\<cdot>u` `a \<sqsubseteq> u`
@@ -377,25 +160,25 @@ case (thunk \<Gamma> x e S)
 
     {
     have "ABinds (delete x \<Gamma>)\<cdot>(env_delete x ae) = ABinds (delete x \<Gamma>)\<cdot>ae" by (rule Abinds_env_cong) simp
-    with `ABinds (delete x \<Gamma>)\<cdot>ae \<squnion> aExp e\<cdot>u \<sqsubseteq> ae`
-    have "ABinds (delete x \<Gamma>)\<cdot>(env_delete x ae) \<squnion> aExp e\<cdot>u \<sqsubseteq> ae" by simp
+    with `ABinds (delete x \<Gamma>)\<cdot>ae \<squnion> Aexp e\<cdot>u \<sqsubseteq> ae`
+    have "ABinds (delete x \<Gamma>)\<cdot>(env_delete x ae) \<squnion> Aexp e\<cdot>u \<sqsubseteq> ae" by simp
     moreover
     from **[folded eq] set_mp[OF artiy_edom_prognosis, unfolded edomIff]
-    have "(ABinds (delete x \<Gamma>)\<cdot>(env_delete x ae) \<squnion> aExp e\<cdot>u) x = \<bottom>" by metis
+    have "(ABinds (delete x \<Gamma>)\<cdot>(env_delete x ae) \<squnion> Aexp e\<cdot>u) x = \<bottom>" by metis
     ultimately
-    have "ABinds (delete x \<Gamma>)\<cdot>(env_delete x ae) \<squnion> aExp e\<cdot>u \<sqsubseteq> env_delete x ae" by (metis below_env_deleteI)
+    have "ABinds (delete x \<Gamma>)\<cdot>(env_delete x ae) \<squnion> Aexp e\<cdot>u \<sqsubseteq> env_delete x ae" by (metis below_env_deleteI)
     }
     moreover
 
 
     have "const_on ae (ap S) (up\<cdot>0)" using thunk by auto
     hence "const_on (env_delete x ae) (ap S) (up\<cdot>0)" using `x \<notin>  ap S`
-      by (auto simp add: const_on_def env_delete_def)
+      by (fastforce simp add:  env_delete_def)
     moreover
 
     have "const_on ae  (upds (restr_stack (edom ae) S)) (up\<cdot>0)" using thunk by auto
     hence "const_on (env_delete x ae) (upds (restr_stack (edom ae) S)) (up\<cdot>0)" using `x \<notin> upds _`
-      by (auto simp add: const_on_def env_delete_def)
+      by (fastforce simp add: env_delete_def)
     ultimately
     have "consistent (env_delete x ae, env_delete x ce, u) (delete x \<Gamma>, e, Upd x # S)" using thunk `a \<sqsubseteq> u`
       by (auto simp add: join_below_iff insert_absorb elim:below_trans)
@@ -408,7 +191,7 @@ case (thunk \<Gamma> x e S)
       by (simp add: map_of_map_transform)
     hence "conf_transform (ae, ce, a) (\<Gamma>, Var x, S) \<Rightarrow>\<^sub>G
            (restrictA (edom ae) (delete x (map_transform Aeta_expand ae (map_transform ccTransform ae \<Gamma>))), Aeta_expand u (ccTransform u e), Upd x # restr_stack (edom ae) S)"
-        by (auto simp add: env_u_com_delete  map_transform_delete delete_map_transform_env_delete insert_absorb restr_delete_twist simp del: restr_delete)
+        by (auto simp add:  map_transform_delete delete_map_transform_env_delete insert_absorb restr_delete_twist simp del: restr_delete)
     also
     have "\<dots> \<Rightarrow>\<^sub>G\<^sup>* (restrictA (edom ae) (delete x (map_transform Aeta_expand ae (map_transform ccTransform ae \<Gamma>))), Aeta_expand u (ccTransform u e), restr_stack (edom ae) S)"
       by (rule r_into_rtranclp, rule)
@@ -417,7 +200,7 @@ case (thunk \<Gamma> x e S)
       by (intro normal_trans Aeta_expand_correct `Astack (restr_stack (edom ae) S) \<sqsubseteq> u`)
     also(rtranclp_trans)
     have "\<dots> = conf_transform (env_delete x ae, env_delete x ce, u) (delete x \<Gamma>, e, Upd x # S)" 
-      by (auto simp add: env_u_com_delete  map_transform_delete delete_map_transform_env_delete insert_absorb restr_delete_twist)
+      by (auto simp add:  map_transform_delete delete_map_transform_env_delete insert_absorb restr_delete_twist)
     finally(back_subst)
     have "conf_transform (ae, ce, a) (\<Gamma>, Var x, S) \<Rightarrow>\<^sub>G\<^sup>* conf_transform (env_delete x ae, env_delete x ce, u) (delete x \<Gamma>, e, Upd x # S)".
     }
@@ -437,7 +220,7 @@ case (thunk \<Gamma> x e S)
     
     have "prognosis ae 0 (delete x \<Gamma>, e, Upd x # S) \<sqsubseteq> ce" using *[unfolded `u=0`] thunk by (auto elim: below_trans)
     moreover
-    note `ABinds (delete x \<Gamma>)\<cdot>ae \<squnion> aExp e\<cdot>u \<sqsubseteq> ae`
+    note `ABinds (delete x \<Gamma>)\<cdot>ae \<squnion> Aexp e\<cdot>u \<sqsubseteq> ae`
     ultimately
     have "consistent (ae, ce, 0) (delete x \<Gamma>, e, Upd x # S)" using thunk `ae x = up\<cdot>u` `u = 0`  by auto
     moreover
@@ -454,15 +237,15 @@ case (thunk \<Gamma> x e S)
 next
 case (lamvar \<Gamma> x e S)
   from lamvar have [simp]: "x \<in> domA \<Gamma>" by auto (metis domI dom_map_of_conv_domA)
-  from lamvar have "aExp (Var x)\<cdot>a \<sqsubseteq> ae" by (auto simp add: join_below_iff)
-  from below_trans[OF aExp_Var fun_belowD[OF this] ]
+  from lamvar have "Aexp (Var x)\<cdot>a \<sqsubseteq> ae" by (auto simp add: join_below_iff)
+  from below_trans[OF Aexp_Var fun_belowD[OF this] ]
   have "up\<cdot>a \<sqsubseteq> ae x".
   then obtain u where "ae x = up\<cdot>u" and "a \<sqsubseteq> u" by (cases "ae x") auto
 
   from Abinds_reorder1[OF `map_of \<Gamma> x = Some e`] `ae x = up\<cdot>u`
-  have "ABinds (delete x \<Gamma>)\<cdot>ae \<squnion> aExp e\<cdot>u = ABinds \<Gamma>\<cdot>ae" by (auto intro: join_comm)
+  have "ABinds (delete x \<Gamma>)\<cdot>ae \<squnion> Aexp e\<cdot>u = ABinds \<Gamma>\<cdot>ae" by (auto intro: join_comm)
   also have "\<dots> \<sqsubseteq> ae" using lamvar by (auto simp add: join_below_iff)
-  finally have "ABinds (delete x \<Gamma>)\<cdot>ae \<squnion> aExp e\<cdot>u \<sqsubseteq> ae".
+  finally have "ABinds (delete x \<Gamma>)\<cdot>ae \<squnion> Aexp e\<cdot>u \<sqsubseteq> ae".
 
   from `ae x = up\<cdot>u` have "ce x \<noteq> \<bottom>" using lamvar by (auto simp add: edom_def)
   then obtain c where "ce x = up\<cdot>c" by (cases "ce x") auto
@@ -476,7 +259,7 @@ case (lamvar \<Gamma> x e S)
   finally have *: "prognosis ae u ((x, e) # delete x \<Gamma>, e, S) \<sqsubseteq> prognosis ae a (\<Gamma>, Var x, S)" by this simp_all
 
   have "consistent (ae, ce, u) ((x, e) # delete x \<Gamma>, e, S)"
-    using lamvar `ABinds (delete x \<Gamma>)\<cdot>ae \<squnion> aExp e\<cdot>u \<sqsubseteq> ae`  `ae x = up\<cdot>u` edom_mono[OF *]
+    using lamvar `ABinds (delete x \<Gamma>)\<cdot>ae \<squnion> Aexp e\<cdot>u \<sqsubseteq> ae`  `ae x = up\<cdot>u` edom_mono[OF *]
     by (auto simp add: join_below_iff split:if_splits intro: below_trans[OF _ `a \<sqsubseteq> u`] below_trans[OF *])
   moreover
 
@@ -542,7 +325,7 @@ case (var\<^sub>2 \<Gamma> x e S)
 next
   case (let\<^sub>1 \<Delta> \<Gamma> e S)
 
-  let ?ae = "aHeap \<Delta> e\<cdot>a"
+  let ?ae = "Aheap \<Delta> e\<cdot>a"
   let ?new = "(domA (\<Delta> @ \<Gamma>) \<union> upds S - (domA \<Gamma> \<union> upds S))"
   have new: "?new = domA \<Delta>"
     using fresh_distinct[OF let\<^sub>1(1)] fresh_distinct_fv[OF let\<^sub>1(2)]
@@ -551,7 +334,7 @@ next
   let ?ce = "fHeap \<Delta> e\<cdot>a"
 
   have "domA \<Delta> \<inter> upds S = {}" using fresh_distinct_fv[OF let\<^sub>1(2)] by (auto dest: set_mp[OF ups_fv_subset])
-  hence *: "\<And> x. x \<in> upds S \<Longrightarrow> x \<notin> edom ?ae" by (auto dest!: set_mp[OF edom_aHeap])
+  hence *: "\<And> x. x \<in> upds S \<Longrightarrow> x \<notin> edom ?ae" by (auto dest!: set_mp[OF edom_Aheap])
 
   have restr_stack_simp: "restr_stack (edom (?ae \<squnion> ae)) S = restr_stack (edom ae) S"
     by (auto intro: restr_stack_cong dest!: *)
@@ -562,47 +345,48 @@ next
     using  fresh_distinct[OF let\<^sub>1(1)] by (auto dest: set_mp[OF ups_fv_subset])
 
   from  fresh_distinct[OF let\<^sub>1(1)]
-   have [simp]: "?ae f|` domA \<Gamma> = \<bottom>" by (auto dest!: set_mp[OF edom_aHeap])
+   have [simp]: "?ae f|` domA \<Gamma> = \<bottom>" by (auto dest!: set_mp[OF edom_Aheap])
 
   {
   have "edom (?ae \<squnion> ae) \<subseteq> domA (\<Delta> @ \<Gamma>) \<union> upds S"
-    using let\<^sub>1(3) by (auto dest: set_mp[OF edom_aHeap])
+    using let\<^sub>1(3) by (auto dest: set_mp[OF edom_Aheap])
   moreover
   (*
   { fix x e'
     assume "map_of \<Delta> x = Some e'"
     hence "x \<notin> edom ae" using `edom ae \<subseteq> - domA \<Delta>` by (metis Compl_iff contra_subsetD domI dom_map_of_conv_domA)
-    hence "fup\<cdot>(aExp e')\<cdot>((?ae \<squnion> ae) x) = fup\<cdot>(aExp e')\<cdot>(?ae x)" by (auto simp add: edomIff)
+    hence "fup\<cdot>(Aexp e')\<cdot>((?ae \<squnion> ae) x) = fup\<cdot>(Aexp e')\<cdot>(?ae x)" by (auto simp add: edomIff)
     also
-    have "fup\<cdot>(aExp e')\<cdot>(?ae x) \<sqsubseteq> (fup\<cdot>(aExp e')\<cdot>(?ae x) f|` domA \<Delta>) \<squnion> (fup\<cdot>(aExp e')\<cdot>(?ae x) f|` (- domA \<Delta>))"
+    have "fup\<cdot>(Aexp e')\<cdot>(?ae x) \<sqsubseteq> (fup\<cdot>(Aexp e')\<cdot>(?ae x) f|` domA \<Delta>) \<squnion> (fup\<cdot>(Aexp e')\<cdot>(?ae x) f|` (- domA \<Delta>))"
       by (rule eq_imp_below[OF join_env_restr_UNIV[symmetric]]) auto
     also
     from `map_of \<Delta> x = Some e'`
-    have "fup\<cdot>(aExp e')\<cdot>(?ae x) f|` domA \<Delta> \<sqsubseteq> ?ae" by (rule aHeap_heap)
+    have "fup\<cdot>(Aexp e')\<cdot>(?ae x) f|` domA \<Delta> \<sqsubseteq> ?ae" by (rule Aheap_heap)
     also
     from `map_of \<Delta> x = Some e'`
-    have "fup\<cdot>(aExp e')\<cdot>(?ae x) f|` (- domA \<Delta>) \<sqsubseteq> aExp (Terms.Let \<Delta> e)\<cdot>a" by (rule aHeap_heap2)
+    have "fup\<cdot>(Aexp e')\<cdot>(?ae x) f|` (- domA \<Delta>) \<sqsubseteq> Aexp (Terms.Let \<Delta> e)\<cdot>a" by (rule Aheap_heap2)
     also
-    have "aExp (Terms.Let \<Delta> e)\<cdot>a \<sqsubseteq> ae" using let\<^sub>1(3) by auto
+    have "Aexp (Terms.Let \<Delta> e)\<cdot>a \<sqsubseteq> ae" using let\<^sub>1(3) by auto
     finally
-    have "fup\<cdot>(aExp e')\<cdot>((?ae \<squnion> ae) x) \<sqsubseteq> ?ae \<squnion> ae" by this auto
+    have "fup\<cdot>(Aexp e')\<cdot>((?ae \<squnion> ae) x) \<sqsubseteq> ?ae \<squnion> ae" by this auto
   }
   moreover
   { fix x e'
     assume "map_of \<Gamma> x = Some e'"
     hence "x \<in> domA \<Gamma>" by (metis domI dom_map_of_conv_domA)
-    hence "x \<notin> edom ?ae" using fresh_distinct[OF let\<^sub>1(1)]  by (auto dest: set_mp[OF edom_aHeap])
+    hence "x \<notin> edom ?ae" using fresh_distinct[OF let\<^sub>1(1)]  by (auto dest: set_mp[OF edom_Aheap])
     moreover
     note let\<^sub>1 `map_of \<Gamma> x = Some e'`
     ultimately
-    have "fup\<cdot>(aExp e')\<cdot>((?ae \<squnion> ae) x) \<sqsubseteq> ae" by (auto simp add: edomIff)
-    hence "fup\<cdot>(aExp e')\<cdot>((?ae \<squnion> ae) x) \<sqsubseteq> ?ae \<squnion> ae" by (metis (erased, hide_lams) "HOLCF-Join-Classes.join_above2" below_trans)
+    have "fup\<cdot>(Aexp e')\<cdot>((?ae \<squnion> ae) x) \<sqsubseteq> ae" by (auto simp add: edomIff)
+    hence "fup\<cdot>(Aexp e')\<cdot>((?ae \<squnion> ae) x) \<sqsubseteq> ?ae \<squnion> ae" by (metis (erased, hide_lams) "HOLCF-Join-Classes.join_above2" below_trans)
   }
   moreover
   *)
   { fix x e'
     assume "x \<in> thunks \<Gamma>"
-    hence "x \<notin> edom ?ce" using fresh_distinct[OF let\<^sub>1(1)]  by (auto dest: set_mp[OF edom_aHeap]  set_mp[OF thunks_domA])
+    hence "x \<notin> edom ?ce" using fresh_distinct[OF let\<^sub>1(1)]
+      by (auto simp add: edom_fHeap dest: set_mp[OF edom_Aheap]  set_mp[OF thunks_domA])
     hence [simp]: "?ce x = \<bottom>" unfolding edomIff by auto
   
     assume "many \<sqsubseteq> (?ce \<squnion> ce) x"
@@ -619,30 +403,19 @@ next
     hence [simp]: "ce x = \<bottom>"  by (auto simp add: edomIff)
 
     assume "many \<sqsubseteq> (?ce \<squnion> ce) x" with `x \<in> thunks \<Delta>`
-    have "(?ae \<squnion> ae) x = up \<cdot> 0" by (auto simp add: aHeap_heap3)
+    have "(?ae \<squnion> ae) x = up \<cdot> 0" by (auto simp add: Aheap_heap3)
   }
   moreover
-  have "const_on ae (ap S) (up\<cdot>0)" using let\<^sub>1 by auto
-  hence "const_on (?ae \<squnion> ae) (ap S) (up\<cdot>0)"  unfolding const_on_def by auto
+  have "const_on ae (ap S) (up\<cdot>0)" using let\<^sub>1 by auto  
+  hence "const_on (?ae \<squnion> ae) (ap S) (up\<cdot>0)" by fastforce
   moreover
   have "const_on ae (upds (restr_stack (edom ae) S)) (up\<cdot>0)" using let\<^sub>1 by auto
-  hence "const_on (?ae \<squnion> ae) (upds (restr_stack (edom ae) S)) (up\<cdot>0)" unfolding const_on_def by auto
+  hence "const_on (?ae \<squnion> ae) (upds (restr_stack (edom ae) S)) (up\<cdot>0)"  by fastforce
   hence "const_on (?ae \<squnion> ae) (upds (restr_stack (edom (?ae \<squnion> ae)) S)) (up\<cdot>0)" unfolding restr_stack_simp.
   moreover
   have "Astack (restr_stack (edom (?ae \<squnion> ae)) S) \<sqsubseteq> a" unfolding restr_stack_simp using let\<^sub>1 by auto
   moreover
-  (*
-  {
-  have "aExp e\<cdot>a \<sqsubseteq> (aExp e\<cdot>a f|` domA \<Delta>) \<squnion> (aExp e\<cdot>a f|` (- domA \<Delta>))"
-    by (rule eq_imp_below[OF join_env_restr_UNIV[symmetric]]) auto
-  also have "aExp e\<cdot>a f|` (- domA \<Delta>) \<sqsubseteq> aExp (Let \<Delta> e)\<cdot>a" by (rule aExp_Let_above)
-  also have "\<dots> \<sqsubseteq> ae" using let\<^sub>1(3) by auto
-  also have "aExp e\<cdot>a f|` domA \<Delta> \<sqsubseteq> ?ae" by (rule aHeap_above_aExp)
-  finally have "aExp e\<cdot>a \<sqsubseteq> ?ae \<squnion> ae" by this auto
-  }
-  moreover
-  *)
-  have "edom (?ce \<squnion> ce) = edom (?ae \<squnion> ae)" using let\<^sub>1 by auto
+  have "edom (?ce \<squnion> ce) = edom (?ae \<squnion> ae)" using let\<^sub>1 by (auto simp add: edom_fHeap)
   moreover
   {
   have "prognosis (?ae \<squnion> ae) a (\<Delta> @ \<Gamma>, e, S) \<sqsubseteq> ?ce \<squnion> prognosis ae a (\<Gamma>, Let \<Delta> e, S)" by (rule prognosis_Let)
@@ -655,19 +428,19 @@ next
   have "heap_upds_ok (\<Delta> @ \<Gamma>, S)" by (rule heap_upds_ok_append)
   moreover
   {
-  have "ABinds \<Delta>\<cdot>(aHeap \<Delta> e\<cdot>a \<squnion> ae) = ABinds \<Delta>\<cdot>(aHeap \<Delta> e\<cdot>a)"
+  have "ABinds \<Delta>\<cdot>(Aheap \<Delta> e\<cdot>a \<squnion> ae) = ABinds \<Delta>\<cdot>(Aheap \<Delta> e\<cdot>a)"
     by (rule Abinds_env_restr_cong) (simp add: env_restr_join)
   moreover
-  have "ABinds \<Gamma>\<cdot>(aHeap \<Delta> e\<cdot>a \<squnion> ae) = ABinds \<Gamma>\<cdot>ae"
+  have "ABinds \<Gamma>\<cdot>(Aheap \<Delta> e\<cdot>a \<squnion> ae) = ABinds \<Gamma>\<cdot>ae"
     by (rule Abinds_env_restr_cong) (simp add: env_restr_join)
   ultimately
-  have "ABinds (\<Delta> @ \<Gamma>) \<cdot> (aHeap \<Delta> e\<cdot>a \<squnion> ae) \<squnion> aExp e\<cdot>a = (ABinds \<Delta>\<cdot>(aHeap \<Delta> e\<cdot>a) \<squnion> aExp e\<cdot>a) \<squnion> ABinds \<Gamma>\<cdot>ae"
+  have "ABinds (\<Delta> @ \<Gamma>) \<cdot> (Aheap \<Delta> e\<cdot>a \<squnion> ae) \<squnion> Aexp e\<cdot>a = (ABinds \<Delta>\<cdot>(Aheap \<Delta> e\<cdot>a) \<squnion> Aexp e\<cdot>a) \<squnion> ABinds \<Gamma>\<cdot>ae"
     apply (simp add: Abinds_append_disjoint[OF fresh_distinct[OF let\<^sub>1(1)]])
     by (metis join_comm)
-  moreover have "(ABinds \<Delta>\<cdot>(aHeap \<Delta> e\<cdot>a) \<squnion> aExp e\<cdot>a) \<sqsubseteq> aHeap \<Delta> e\<cdot>a \<squnion> aExp (Let \<Delta> e)\<cdot>a" by (rule aExp_Let)
-  moreover have " ABinds \<Gamma>\<cdot>ae \<squnion> aExp (Let \<Delta> e)\<cdot>a \<sqsubseteq> ae" using let\<^sub>1 by auto
+  moreover have "(ABinds \<Delta>\<cdot>(Aheap \<Delta> e\<cdot>a) \<squnion> Aexp e\<cdot>a) \<sqsubseteq> Aheap \<Delta> e\<cdot>a \<squnion> Aexp (Let \<Delta> e)\<cdot>a" by (rule Aexp_Let)
+  moreover have " ABinds \<Gamma>\<cdot>ae \<squnion> Aexp (Let \<Delta> e)\<cdot>a \<sqsubseteq> ae" using let\<^sub>1 by auto
   ultimately
-  have "ABinds (\<Delta> @ \<Gamma>) \<cdot> (aHeap \<Delta> e\<cdot>a \<squnion> ae) \<squnion> aExp e\<cdot>a \<sqsubseteq> aHeap \<Delta> e\<cdot>a \<squnion> ae"
+  have "ABinds (\<Delta> @ \<Gamma>) \<cdot> (Aheap \<Delta> e\<cdot>a \<squnion> ae) \<squnion> Aexp e\<cdot>a \<sqsubseteq> Aheap \<Delta> e\<cdot>a \<squnion> ae"
     apply (simp only: join_assoc[symmetric])
     apply (erule below_trans[OF join_mono[OF _ below_refl]])
     apply (simp only: join_assoc)
@@ -682,7 +455,7 @@ next
   {
     have "\<And> x. x \<in> domA \<Gamma> \<Longrightarrow> x \<notin> edom ?ae"
       using fresh_distinct[OF let\<^sub>1(1)]
-      by (auto dest!: set_mp[OF edom_aHeap])
+      by (auto dest!: set_mp[OF edom_Aheap])
     hence "restrictA (edom (?ae \<squnion> ae)) (map_transform Aeta_expand (?ae \<squnion> ae) (map_transform transform (?ae \<squnion> ae) \<Gamma>))
        = restrictA (edom ae) (map_transform Aeta_expand ae (map_transform transform ae \<Gamma>))"
        by (auto intro!: map_transform_cong restrictA_cong simp add: edomIff)
@@ -699,7 +472,7 @@ next
 
     have "conf_transform (ae, ce, a) (\<Gamma>, Let \<Delta> e, S) \<Rightarrow>\<^sub>G\<^sup>* conf_transform (?ae \<squnion> ae, ?ce \<squnion> ce, a) (\<Delta> @ \<Gamma>, e, S)"
       using restr_stack_simp let\<^sub>1(1,2)
-      by (fastforce intro!: lam_and_restrict simp  add: map_transform_append restrictA_append restr_stack_simp   dest: set_mp[OF edom_aHeap])
+      by (fastforce intro!: lam_and_restrict simp  add: map_transform_append restrictA_append restr_stack_simp   dest: set_mp[OF edom_Aheap])
   }
   ultimately
   show ?case by (blast del: consistentI consistentE)
@@ -716,7 +489,7 @@ next
 qed
 
 
-
+end
 
 
 end
