Launchbury/ArityStack.thy
@@ -1,0 +1,15 @@
+theory ArityStack
+imports "Arity" SestoftConf
+begin
+
+fun Astack :: "stack \<Rightarrow> Arity"
+  where "Astack [] = 0"
+      | "Astack (Arg x # S) = inc\<cdot>(Astack S)"
+      | "Astack (Upd x # S) = 0"
+      | "Astack (Dummy x # S) = 0"
+
+lemma Astack_restr_stack_below:
+  "Astack (restr_stack V S) \<sqsubseteq> Astack S"
+  by (induction V S rule: restr_stack.induct) auto
+
+end
