Launchbury/Cardinality-Domain.thy
@@ -1,0 +1,45 @@
+theory "Cardinality-Domain"
+imports "HOLCF-Utils"
+begin
+
+type_synonym oneShot = "one"
+abbreviation notOneShot :: oneShot where "notOneShot \<equiv> ONE"
+abbreviation oneShot :: oneShot where "oneShot \<equiv> \<bottom>"
+
+type_synonym two = "oneShot\<^sub>\<bottom>"
+abbreviation many :: two where "many \<equiv> up\<cdot>notOneShot"
+abbreviation once :: two where "once \<equiv> up\<cdot>oneShot"
+abbreviation none :: two where "none \<equiv> \<bottom>"
+
+lemma two_conj: "c = many \<or> c = once \<or> c = none" by (metis Exh_Up one_neq_iffs(1))
+
+lemma two_cases[case_names many once none]:
+  obtains "c = many" | "c = once" | "c = none" using two_conj by metis
+
+definition two_pred where "two_pred = (\<Lambda> x. if x \<sqsubseteq> once then \<bottom> else x)"
+
+lemma two_pred_simp: "two_pred\<cdot>c = (if c \<sqsubseteq> once then \<bottom> else c)"
+  unfolding two_pred_def
+  apply (rule beta_cfun)
+  apply (rule cont_if_else_above)
+  apply (auto elim: below_trans)
+  done
+
+lemma two_pred_below_arg: "two_pred \<cdot> f \<sqsubseteq> f"
+  by (auto simp add: two_pred_simp)
+
+lemma two_pred_none: "two_pred\<cdot>c = none \<longleftrightarrow> c \<sqsubseteq> once"
+  by (auto simp add: two_pred_simp)
+
+definition record_call where "record_call x = (\<Lambda> ce. (\<lambda> y. if x = y then two_pred\<cdot>(ce y) else ce y))"
+
+lemma record_call[simp]: "(record_call x \<cdot> f) x = two_pred \<cdot> (f x)"
+  unfolding record_call_def by auto
+
+lemma record_call_below_arg: "record_call x \<cdot> f \<sqsubseteq> f"
+  unfolding record_call_def
+  by (auto intro!: fun_belowI two_pred_below_arg)
+
+
+
+end
