Launchbury/Env.thy
@@ -61,11 +61,12 @@ abbreviation env_restr_rev  (infixl "f|`"  110) where "env_restr_rev m S \<equiv
 
 notation (latex output) env_restr_rev ("_|\<^bsub>_\<^esub>")
 
-lemma env_restr_empty[simp]: "m f|` S = \<bottom> \<longleftrightarrow> edom m \<inter> S = {}"
+lemma env_restr_empty_iff[simp]: "m f|` S = \<bottom> \<longleftrightarrow> edom m \<inter> S = {}"
   apply (auto simp add: edom_def env_restr_def lambda_strict[symmetric]  split:if_splits)
   apply metis
   apply (fastforce simp add: edom_def env_restr_def lambda_strict[symmetric]  split:if_splits)
   done
+lemmas iffD2[OF env_restr_empty_iff, simp]
 
 lemma lookup_env_restr[simp]: "x \<in> S \<Longrightarrow> (m f|` S) x = m x"
   by (fastforce simp add: env_restr_def)
