ROOT
@@ -33,10 +33,11 @@ session LaunchburyComplete (AFP) in "Launchbury" = "HOLCF-Nominal2" +
 session Arity (AFP) in "Launchbury" = "HOLCF-Nominal2" +
   options [document_variants = arity, document = pdf, document_graph, document_output = "output" ]
   theories
-    "ArityCorrect2"
+    "ArityCorrectLaunchbury"
     "ArityAnalysisImpl"
     "TrivialArityAnal"
     "ArityEtaExpand"
+    "FutureEtaExpand"
     "EtaExpansionSestoft"
     "DeadCodeRemovalCorrect"
     "DeadCodeRemoval2Correct"
